code/ecdsa/Hacl.Impl.EC.MontgomeryMultiplication.Lemmas.fst
@@ -1,52 +1,32 @@
 module Hacl.Impl.EC.MontgomeryMultiplication.Lemmas
 
-
-open FStar.HyperStack.All
-open FStar.HyperStack
-module ST = FStar.HyperStack.ST
-
-open Hacl.Impl.P256.Math 
-
 open Lib.IntTypes
-open Lib.Buffer
 
 open FStar.Math.Lemmas
 open FStar.Mul
 
-open Hacl.Spec.EC.Definition
 open Hacl.Lemmas.P256
 open Spec.ECC
 open Spec.ECC.Curves
-open Spec.ECDSA.Lemmas
 
-open Hacl.Impl.EC.LowLevel
-
-open Lib.Loops
 open Hacl.Spec.MontgomeryMultiplication
 open Hacl.Impl.EC.Setup
 
 
-#set-options "--z3rlimit 200"
+#set-options "--z3rlimit 200 --ifuel 0 --fuel 0"
 
 open Lib.Sequence
 
-val lemma_mod_inv: #c: curve ->  t: int -> Lemma (t % getPrime c = t * modp_inv2 #c (pow2 0) % getPrime c)
+val lemma_mod_inv: #c: curve -> t: int -> Lemma (t % getPrime c = t * modp_inv2 #c (pow2 0) % getPrime c)
 
 let lemma_mod_inv #c t = 
   let prime = getPrime c in 
   lemma_pow_mod_n_is_fpow prime 1 (prime - 2);
   power_one (prime - 2)
 
-
-open FStar.Math.Euclid 
-open FStar.Math.Fermat
-
-
-#push-options "--z3rlimit 100 --ifuel 0 --fuel 0"
-
 val lemma_division_is_multiplication:
-  t3: nat{t3 % pow2 64 = 0} ->
-  prime: pos {is_prime prime /\ prime > 3 /\ prime > pow2 64} -> 
+  t3: nat{t3 % pow2 64 = 0} -> 
+  prime: pos {FStar.Math.Euclid.is_prime prime /\ prime > 3 /\ prime > pow2 64} -> 
   Lemma (t3 * modp_inv2_prime (pow2 64) prime % prime = (t3 / pow2 64) % prime)
 
 let lemma_division_is_multiplication t3 prime =  
@@ -112,11 +92,6 @@ let lemma_k0_computation #c t k0 =
   
   assert(k % pow2 64 == 0)
 
-
-
-
-
-
 val montgomery_multiplication_one_round_proof: 
   #c: curve ->
   t: nat ->
@@ -133,17 +108,12 @@ let montgomery_multiplication_one_round_proof #c t k0 round co =
   let k = t + prime * (((t % pow2 64) * v k0) % pow2 64) in 
 
   lemma_k0_computation #c t k0;
-  assume (is_prime prime /\ prime > pow2 64);
   lemma_division_is_multiplication k prime;
 
   modulo_addition_lemma t prime (((t % pow2 64) * v k0) % pow2 64);
 
   lemma_mod_mul_distr_l k (modp_inv2_prime (pow2 64) prime) prime;
   lemma_mod_mul_distr_l co (modp_inv2_prime (pow2 64) prime) prime
-
-
-
-
 
 
 val lemma_up_bound0: #c: curve -> t0: nat {t0 < getPrime c * pow2 (64 * v (getCoordinateLenU64 c))} 
@@ -153,6 +123,8 @@ val lemma_up_bound0: #c: curve -> t0: nat {t0 < getPrime c * pow2 (64 * v (getCo
 let lemma_up_bound0 #c t0 t = 
   let prime = getPrime c in 
   let s = pow2 (64 * v (getCoordinateLenU64 c)) in 
+  assert(getPower c == v (getCoordinateLenU64 c) * 64);
+  assert(prime < pow2 (v (getCoordinateLenU64 c) * 64));
   lemma_mult_lt_left prime prime s;
   assert(t0 < prime * s);
   assert(t0 / s < prime);
@@ -191,20 +163,17 @@ let lemma_mm_reduction #c a0 i =
   let open Spec.ECC in 
   let prime = getPrime c in 
   
-  let a = pow2 (i * 64) in 
+  let a = pow2 (i * 64) in
+  let exp_prime: pos = prime - 2 in
 
-  let exp_prime: pos = prime - 2 in 
-
-  assert(modp_inv2 #c a == exp #prime (a % prime) exp_prime % prime);
+  assert(modp_inv2 #c a == exp #prime (a % prime) (prime - 2));
+  
   Hacl.Lemmas.P256.lemma_pow_mod_n_is_fpow prime (a % prime) exp_prime;
-  lemma_mod_twice (pow (a % prime) exp_prime) prime;
 
-  assert(modp_inv2 #c (pow2 64) == exp #prime (pow2 64 % prime) exp_prime % prime);
+  assert(modp_inv2 #c (pow2 64) == exp #prime (pow2 64 % prime) exp_prime);
   Hacl.Lemmas.P256.lemma_pow_mod_n_is_fpow prime (pow2 64 % prime) exp_prime;
-  lemma_mod_twice (pow (pow2 64 % prime) exp_prime) prime;
 
   Hacl.Lemmas.P256.power_distributivity_2 (a % prime) (pow2 64 % prime) exp_prime;
-
 
   lemma_mod_mul_distr_r a0 (modp_inv2 #c a * modp_inv2 #c (pow2 64)) prime;
 
@@ -219,7 +188,7 @@ let lemma_mm_reduction #c a0 i =
     (==) {pow_plus (a % prime) (pow2 64 % prime) exp_prime}
     (pow (a % prime * (pow2 64 % prime)) exp_prime) % prime; 
     (==) {Hacl.Lemmas.P256.power_distributivity (a % prime * (pow2 64 % prime)) exp_prime prime}
-    (pow (a % prime * (pow2 64 % prime) % prime) exp_prime) % prime; 
+    (pow (a % prime * (pow2 64 % prime) % prime) exp_prime) % prime;  
     (==) {lemma_mod_mul_distr_l a (pow2 64 % prime) prime}
     (pow ((a * (pow2 64 % prime)) % prime) exp_prime) % prime; 
     (==) {lemma_mod_mul_distr_r a (pow2 64) prime}
@@ -229,9 +198,12 @@ let lemma_mm_reduction #c a0 i =
     (==) {Hacl.Lemmas.P256.lemma_pow_mod_n_is_fpow prime (a * pow2 64 % prime) exp_prime} 
     exp #prime ((a * pow2 64) % prime) exp_prime % prime; 
     (==) {}
-    modp_inv2 #c (a * pow2 64);
+    modp_inv2 #c (a * pow2 64) % prime; 
+    (==) {small_mod (modp_inv2 #c (a * pow2 64)) prime}
+    modp_inv2 #c (a * pow2 64); 
     (==) {pow2_plus (i * 64) 64}
-    modp_inv2 #c (pow2 ((i + 1) * 64));};
+    modp_inv2 #c (pow2 ((i + 1) * 64)); 
+    };
 
   let open FStar.Tactics in 
   let open FStar.Tactics.Canon in 
@@ -250,10 +222,10 @@ let lemma_mult_lt_center a b c d = ()
 
 val lemma_domain: #c: curve -> #m: mode -> a: nat {a < getModePrime m c} -> b: nat {b < getModePrime m c} ->  k: nat ->
   Lemma 
-    (requires (k == (a *  b * modp_inv2_prime (pow2 (getPower c)) (getModePrime m c)) % getModePrime m c))
-    (ensures (
-      k == toDomain_ #c #m (fromDomain_ #c #m a * fromDomain_ #c #m b % getModePrime m c) /\
-      k == toDomain_ #c #m (fromDomain_ #c #m a * fromDomain_ #c #m b)))
+  (requires (k == (a *  b * modp_inv2_prime (pow2 (getPower c)) (getModePrime m c)) % getModePrime m c))
+  (ensures (
+    k == toDomain_ #c #m (fromDomain_ #c #m a * fromDomain_ #c #m b % getModePrime m c) /\
+    k == toDomain_ #c #m (fromDomain_ #c #m a * fromDomain_ #c #m b)))
 
 let lemma_domain #c #m a b k = 
   let prime = getModePrime m c in 
